

Problem 1

Hand-in 1 Jonatan Haraldsson

Show that the MAP using the likelihood $p(d|\theta) = \mathcal{N}(d; [\Phi\theta]_i, \sigma^2)$ and the prior: $p(\theta) = \prod_{i=1}^M \mathcal{N}(\theta_i; 0, \sigma_i^2)$

is equal to $\hat{\theta}_{\text{ridge}} = \underset{\theta}{\operatorname{argmin}} \{ (\Phi\theta - D)^T (\Phi\theta - D) + \lambda \sum_{i=1}^M \theta_i^2 \}$

The likelihood is given by $p(D|\theta) = \mathcal{N}(D|\Phi\theta, \sigma^2) = \left(\frac{1}{2\pi\sigma^2}\right)^{N/2} \exp\left\{-\frac{1}{2} \frac{(D-\Phi\theta)^T (D-\Phi\theta)}{\sigma^2}\right\}$

Similarly the prior is given by: $p(\theta) = \prod_{i=1}^M \mathcal{N}(\theta_i; 0, \sigma_i^2) = \prod_{i=1}^M \sqrt{\frac{1}{2\pi\sigma_i^2}} \exp\left\{-\frac{1}{2} \frac{\theta_i^2}{\sigma_i^2}\right\} = \left[\frac{1}{2\pi\sigma_i^2}\right]^{M/2} \exp\left\{-\frac{1}{2\sigma_i^2} \sum_{i=1}^M \theta_i^2\right\}$

From Bayes' the posterior \propto "likelihood \times prior". Thus, $\hat{\theta}_{\text{MAP}} = \underset{\theta}{\operatorname{argmax}} \{ p(D|\theta) p(\theta) \}$.

Let's go!

$$p(D|\theta) p(\theta) = \left(\frac{1}{2\pi\sigma^2}\right)^{N/2} \exp\left\{-\frac{1}{2} \frac{(D-\Phi\theta)^T (D-\Phi\theta)}{\sigma^2}\right\} \left[\frac{1}{2\pi\sigma_i^2}\right]^{M/2} \exp\left\{-\frac{1}{2\sigma_i^2} \sum_{i=1}^M \theta_i^2\right\} \sim \left\{ \begin{array}{l} \text{No } \theta \text{ dependence in the pre-factors,} \\ \text{so I'll only focus on the exponentials} \end{array} \right\}$$

$$p(D|\theta) p(\theta) \sim \exp\left\{-\frac{1}{2} \frac{(D-\Phi\theta)^T (D-\Phi\theta)}{\sigma^2}\right\} \exp\left\{-\frac{1}{2\sigma_i^2} \sum_{i=1}^M \theta_i^2\right\} = \exp\left\{-\frac{1}{2\sigma^2} [(D-\Phi\theta)^T (D-\Phi\theta)] - \frac{1}{2\sigma_i^2} \sum_{i=1}^M \theta_i^2\right\} =$$

$$= \left\{ \frac{\text{Factor-out}}{\frac{1}{2\sigma^2}} \right\} = \exp\left\{-\frac{1}{2\sigma^2} [(D-\Phi\theta)^T (D-\Phi\theta) + \sigma^2 \sum_{i=1}^M \theta_i^2]\right\} = e^{-f(\theta)}$$

$$\text{Finding } \underset{\theta}{\operatorname{argmax}} \{ p(D|\theta) p(\theta) \} \Leftrightarrow \underset{\theta}{\operatorname{argmax}} \{ e^{-f(\theta)} \} \stackrel{= f(\theta)}{\Leftrightarrow} \left\{ e^{-f(\theta)} \text{ is max for min}\{f(\theta)\} \right\} \Leftrightarrow \underset{\theta}{\operatorname{argmin}} \{ f(\theta) \}$$

$$\text{To wrap up: } \hat{\theta}_{\text{MAP}} = \underset{\theta}{\operatorname{argmax}} \{ p(D|\theta) p(\theta) \} = \underset{\theta}{\operatorname{argmin}} \{ f(\theta) \} = \left\{ \begin{array}{l} \text{Again, excluding} \\ \text{the } -\frac{1}{2\sigma^2} \text{ pre-factor} \end{array} \right\} = \underset{\theta}{\operatorname{argmin}} \{ (D-\Phi\theta)^T (D-\Phi\theta) + \sigma^2 \sum_{i=1}^M \theta_i^2 \}$$

$$\text{Comparing to where I'm supposed to arrive, } \lambda = \left(\frac{\sigma^2}{\sigma_i^2}\right)^2 \Rightarrow \hat{\theta} = \underset{\theta}{\operatorname{argmin}} \{ (D-\Phi\theta)^T (D-\Phi\theta) + \lambda \sum_{i=1}^M \theta_i^2 \}.$$

Problem 2

Show that the MAP using the likelihood $p(d|\theta) = \mathcal{N}(d; [\Phi\theta]_i, \sigma^2)$ and the prior: $p(\theta) = \prod_{i=1}^M \mathcal{L}(\theta_i; 0, \alpha_i)$

is equal to $\hat{\theta}_{\text{Lasso}} = \underset{\theta}{\operatorname{argmin}} \{ (\Phi\theta - D)^T (\Phi\theta - D) + \lambda \sum_{i=1}^M |\theta_i| \}$

I'll be following the same approach as in problem 1, i.e. finding $\underset{\theta}{\operatorname{argmax}} \{ p(D|\theta) p(\theta) \}$

Course book Ch. 3.2, p.66

We've got the same likelihood, however, the prior is given by: $p(\theta) = \prod_{i=1}^M \mathcal{L}(\theta_i; 0, \alpha_i)$, $\mathcal{L}(\theta_i; 0, \alpha_i) \propto \exp\left\{-\frac{|\theta_i|}{\alpha_i}\right\}$

The prior is then: $p(\theta) \propto \prod_{i=1}^M \mathcal{L}(\theta_i; 0, \alpha_i) = \prod_{i=1}^M \exp\left\{-\frac{|\theta_i|}{\alpha_i}\right\} = \exp\left\{-\frac{1}{\alpha_i} \sum_{i=1}^M |\theta_i|\right\}$

$$\text{Again, omitting the } \theta\text{-independent prefactors: } p(D|\theta) p(\theta) \propto \exp\left\{-\frac{1}{2} \frac{(D-\Phi\theta)^T (D-\Phi\theta)}{\sigma^2}\right\} \exp\left\{-\frac{1}{\alpha_i} \sum_{i=1}^M |\theta_i|\right\} =$$

$$= \exp\left\{-\frac{1}{2\sigma^2} [(D-\Phi\theta)^T (D-\Phi\theta) + \frac{2\sigma^2}{\alpha_i} \sum_{i=1}^M |\theta_i|]\right\}$$

$$\text{Yet again, } \underset{\theta}{\operatorname{argmax}} \left\{ \exp\left\{-\frac{1}{2\sigma^2} [(D-\Phi\theta)^T (D-\Phi\theta) + \frac{2\sigma^2}{\alpha_i} \sum_{i=1}^M |\theta_i|]\right\} \right\} \Leftrightarrow \underset{\theta}{\operatorname{argmin}} \left\{ (D-\Phi\theta)^T (D-\Phi\theta) + \frac{2\sigma^2}{\alpha_i} \sum_{i=1}^M |\theta_i| \right\}$$

Comparing to what I want $\lambda = \frac{2\sigma^2}{\alpha_i}$ in this case.